DUDAS.  
Ejercicio 5 -> ii.  
Ejercicio 6 -> viii.  
Ejercicio 8 -> iii, xi, xii.  


Borrador.  
```
8. iii.
\item Por inducci√≥n en $m$: \\
    $\bullet$ $\hspace{0.01cm}$ Caso base: si $m=0$, ${\mathcal{L}}^n\cdot{\mathcal{L}}^0 = {\mathcal{L}}^n\cdot \Lambda = \mathcal{L}^n = \mathcal{L}^{n+0}$. \\
    $\bullet$ $\hspace{0.01cm}$ Caso inductivo: \\
    Supongo que para $m \geq 0$ se cumple que: $\mathcal{L}^n \cdot \mathcal{L}^m = \mathcal{L}^{n+m}$. Y, quiero ver que se cumple para $m + 1$, es decir: $\mathcal{L}^n \cdot \mathcal{L}^{m+1} = \mathcal{L}^{n+m+1}$. \\
```
